theories/dyn_type.v
@@ -8,37 +8,37 @@ Set Implicit Arguments.
 Unset Strict Implicit.
 Unset Printing Implicit Defensive.
 
-Reserved Notation "Γ ; Δ ⊨ m : A" (at level 50, m, A at next level).
+Reserved Notation "Γ ; Δ ⊢ m : A" (at level 50, Δ, m, A at next level).
 Inductive dyn_type : sta_ctx -> dyn_ctx -> term -> term -> Prop :=
 | dyn_var Γ Δ x A :
   sta_has Γ x A ->
   dyn_has Δ x A ->
-  Γ ; Δ ⊨ Var x : A
+  Γ ; Δ ⊢ Var x : A
 | dyn_lam0 Γ Δ A B m s t :
   Δ ▷ t ->
   Γ ⊢ Pi0 A B s t : @t ->
-  (A :: Γ) ; (_: Δ) ⊨ m : B ->
-  Γ ; Δ ⊨ Lam0 A m s t : Pi0 A B s t
+  (A :: Γ) ; (_: Δ) ⊢ m : B ->
+  Γ ; Δ ⊢ Lam0 A m s t : Pi0 A B s t
 | dyn_lam1 Γ Δ A B m s t :
   Δ ▷ t ->
   Γ ⊢ Pi1 A B s t : @t ->
-  (A :: Γ) ; (A :{s} Δ) ⊨ m : B ->
-  Γ ; Δ ⊨ Lam1 A m s t : Pi1 A B s t
+  (A :: Γ) ; (A :{s} Δ) ⊢ m : B ->
+  Γ ; Δ ⊢ Lam1 A m s t : Pi1 A B s t
 | dyn_app0 Γ Δ A B m n s t :
-  Γ ; Δ ⊨ m : Pi0 A B s t ->
+  Γ ; Δ ⊢ m : Pi0 A B s t ->
   Γ ⊢ n : A ->
-  Γ ; Δ ⊨ App m n : B.[n/]
+  Γ ; Δ ⊢ App m n : B.[n/]
 | dyn_app1 Γ Δ1 Δ2 Δ A B m n s t :
   Δ1 ∘ Δ2 => Δ ->
-  Γ ; Δ1 ⊨ m : Pi1 A B s t ->
-  Γ ; Δ2 ⊨ n : A ->
-  Γ ; Δ ⊨ App m n : B.[n/]
+  Γ ; Δ1 ⊢ m : Pi1 A B s t ->
+  Γ ; Δ2 ⊢ n : A ->
+  Γ ; Δ ⊢ App m n : B.[n/]
 | dyn_conv Γ Δ A B m s :
   A === B ->
-  Γ ; Δ ⊨ m : A ->
+  Γ ; Δ ⊢ m : A ->
   Γ ⊢ B : @s ->
-  Γ ; Δ ⊨ m : B
-where "Γ ; Δ ⊨ m : A" := (dyn_type Γ Δ m A).
+  Γ ; Δ ⊢ m : B
+where "Γ ; Δ ⊢ m : A" := (dyn_type Γ Δ m A).
 
 Inductive dyn_wf : sta_ctx -> dyn_ctx -> Prop :=
 | dyn_wf_nil : dyn_wf nil nil
