theories/era_inv.v
@@ -7,7 +7,7 @@ Unset Strict Implicit.
 Unset Printing Implicit Defensive.
 
 Lemma era_lam0_form Γ Δ m n X B s t :
-  Γ ; Δ ⊨ m ~ Lam0 X n s t : B -> exists A n, m = Lam0 A n s t.
+  Γ ; Δ ⊢ m ~ Lam0 X n s t : B -> exists A n, m = Lam0 A n s t.
 Proof.
   move e:(Lam0 X n s t)=>x er. elim: er X n s t e=>//{Γ Δ m x B}.
   move=>Γ Δ A B m m' s t k tyP er ih X n s0 t0 [e1 e2 e3 e4]; subst.
@@ -15,22 +15,22 @@ Proof.
 Qed.
 
 Lemma era_lam1_form Γ Δ m n X B s t :
-  Γ ; Δ ⊨ m ~ Lam1 X n s t : B -> exists A n, m = Lam1 A n s t.
+  Γ ; Δ ⊢ m ~ Lam1 X n s t : B -> exists A n, m = Lam1 A n s t.
 Proof.
   move e:(Lam1 X n s t)=>x er. elim: er X n s t e=>//{Γ Δ m x B}.
   move=>Γ Δ A B m m' s t k tyP er ih X n s0 t0 [e1 e2 e3 e4]; subst.
   exists A. by exists m.
 Qed.
 
-Lemma era_box_form Γ Δ m A : ~Γ ; Δ ⊨ m ~ Box : A.
+Lemma era_box_form Γ Δ m A : ~Γ ; Δ ⊢ m ~ Box : A.
 Proof. move e:(Box)=>m' ty. elim: ty e=>//{Γ Δ m m' A}. Qed.
 
 Lemma era_lam0_invX Γ Δ A1 A2 A3 B C m1 m2 s1 s2 t1 t2 r :
   dyn_wf (A3 :: Γ) (_: Δ) ->
-  Γ ; Δ ⊨ Lam0 A1 m1 s1 t1 ~ Lam0 A2 m2 s1 t1 : C ->
+  Γ ; Δ ⊢ Lam0 A1 m1 s1 t1 ~ Lam0 A2 m2 s1 t1 : C ->
   C === Pi0 A3 B s2 t2 ->
   (A3 :: Γ) ⊢ B : @r ->
-  (A3 :: Γ) ; _: Δ ⊨ m1 ~ m2 : B /\ s1 = s2 /\ t1 = t2.
+  (A3 :: Γ) ; _: Δ ⊢ m1 ~ m2 : B /\ s1 = s2 /\ t1 = t2.
 Proof with eauto.
   move e1:(Lam0 A1 m1 s1 t1)=>n1.
   move e2:(Lam0 A2 m2 s1 t1)=>n2 wf tyL.
@@ -54,10 +54,10 @@ Qed.
 
 Lemma era_lam1_invX Γ Δ A1 A2 A3 B C m1 m2 s1 s2 t1 t2 r :
   dyn_wf (A3 :: Γ) (A3 :{s2} Δ) ->
-  Γ ; Δ ⊨ Lam1 A1 m1 s1 t1 ~ Lam1 A2 m2 s1 t1 : C ->
+  Γ ; Δ ⊢ Lam1 A1 m1 s1 t1 ~ Lam1 A2 m2 s1 t1 : C ->
   C === Pi1 A3 B s2 t2 ->
   (A3 :: Γ) ⊢ B : @r ->
-  (A3 :: Γ) ; A3 :{s2} Δ ⊨ m1 ~ m2 : B /\ s1 = s2 /\ t1 = t2.
+  (A3 :: Γ) ; A3 :{s2} Δ ⊢ m1 ~ m2 : B /\ s1 = s2 /\ t1 = t2.
 Proof with eauto.
   move e1:(Lam1 A1 m1 s1 t1)=>n1.
   move e2:(Lam1 A2 m2 s1 t1)=>n2 wf tyL.
@@ -82,8 +82,8 @@ Qed.
 Lemma era_lam0_inv Γ Δ m m' A1 A2 A3 B s1 s2 t1 t2 x :
   dyn_wf Γ Δ ->
   Γ ⊢ Pi0 A1 B s1 t1 : @x ->
-  Γ ; Δ ⊨ Lam0 A2 m s2 t2 ~ Lam0 A3 m' s2 t2 : Pi0 A1 B s1 t1 ->
-  (A1 :: Γ) ; _: Δ ⊨ m ~ m' : B /\ s2 = s1 /\ t2 = t1.
+  Γ ; Δ ⊢ Lam0 A2 m s2 t2 ~ Lam0 A3 m' s2 t2 : Pi0 A1 B s1 t1 ->
+  (A1 :: Γ) ; _: Δ ⊢ m ~ m' : B /\ s2 = s1 /\ t2 = t1.
 Proof with eauto.
   move=>wf/sta_pi0_inv[r[tyA1[tyB _]]] tyL.
   apply: era_lam0_invX...
@@ -93,8 +93,8 @@ Qed.
 Lemma era_lam1_inv Γ Δ m m' A1 A2 A3 B s1 s2 t1 t2 x :
   dyn_wf Γ Δ ->
   Γ ⊢ Pi1 A1 B s1 t1 : @x ->
-  Γ ; Δ ⊨ Lam1 A2 m s2 t2 ~ Lam1 A3 m' s2 t2 : Pi1 A1 B s1 t1 ->
-  (A1 :: Γ) ; A1 :{s1} Δ ⊨ m ~ m' : B /\ s2 = s1 /\ t2 = t1.
+  Γ ; Δ ⊢ Lam1 A2 m s2 t2 ~ Lam1 A3 m' s2 t2 : Pi1 A1 B s1 t1 ->
+  (A1 :: Γ) ; A1 :{s1} Δ ⊢ m ~ m' : B /\ s2 = s1 /\ t2 = t1.
 Proof with eauto.
   move=>wf/sta_pi1_inv[r[tyA1[tyB _]]] tyL.
   apply: era_lam1_invX...
