theories/era_type.v
@@ -6,44 +6,44 @@ Set Implicit Arguments.
 Unset Strict Implicit.
 Unset Printing Implicit Defensive.
 
-Reserved Notation "Γ ; Δ ⊨ m ~ n : A" (at level 50, m, n, A at next level).
+Reserved Notation "Γ ; Δ ⊢ m ~ n : A" (at level 50, Δ, m, n, A at next level).
 Inductive era_type : sta_ctx -> dyn_ctx -> term -> term -> term -> Prop :=
 | era_var Γ Δ x A :
   sta_has Γ x A ->
   dyn_has Δ x A ->
-  Γ ; Δ ⊨ Var x ~ Var x : A
+  Γ ; Δ ⊢ Var x ~ Var x : A
 | era_lam0 Γ Δ A B m m' s t :
   Δ ▷ t ->
   Γ ⊢ Pi0 A B s t : @t ->
-  (A :: Γ) ; _: Δ ⊨ m ~ m' : B ->
-  Γ ; Δ ⊨ Lam0 A m s t ~ Lam0 Box m' s t : Pi0 A B s t
+  (A :: Γ) ; _: Δ ⊢ m ~ m' : B ->
+  Γ ; Δ ⊢ Lam0 A m s t ~ Lam0 Box m' s t : Pi0 A B s t
 | era_lam1 Γ Δ A B m m' s t :
   Δ ▷ t ->
   Γ ⊢ Pi1 A B s t : @t ->
-  (A :: Γ) ; A :{s} Δ ⊨ m ~ m' : B ->
-  Γ ; Δ ⊨ Lam1 A m s t ~ Lam1 Box m' s t : Pi1 A B s t
+  (A :: Γ) ; A :{s} Δ ⊢ m ~ m' : B ->
+  Γ ; Δ ⊢ Lam1 A m s t ~ Lam1 Box m' s t : Pi1 A B s t
 | era_app0 Γ Δ A B m m' n s t :
-  Γ ; Δ ⊨ m ~ m' : Pi0 A B s t ->
+  Γ ; Δ ⊢ m ~ m' : Pi0 A B s t ->
   Γ ⊢ n : A ->
-  Γ ; Δ ⊨ App m n ~ App m' Box : B.[n/]
+  Γ ; Δ ⊢ App m n ~ App m' Box : B.[n/]
 | era_app1 Γ Δ1 Δ2 Δ A B m m' n n' s t :
   Δ1 ∘ Δ2 => Δ ->
-  Γ ; Δ1 ⊨ m ~ m' : Pi1 A B s t ->
-  Γ ; Δ2 ⊨ n ~ n' : A ->
-  Γ ; Δ ⊨ App m n ~ App m' n' : B.[n/]
+  Γ ; Δ1 ⊢ m ~ m' : Pi1 A B s t ->
+  Γ ; Δ2 ⊢ n ~ n' : A ->
+  Γ ; Δ ⊢ App m n ~ App m' n' : B.[n/]
 | era_conv Γ Δ A B m m' s :
   A === B ->
-  Γ ; Δ ⊨ m ~ m' : A ->
+  Γ ; Δ ⊢ m ~ m' : A ->
   Γ ⊢ B : @s ->
-  Γ ; Δ ⊨ m ~ m' : B
-where "Γ ; Δ ⊨ m ~ n : A" := (era_type Γ Δ m n A).
+  Γ ; Δ ⊢ m ~ m' : B
+where "Γ ; Δ ⊢ m ~ n : A" := (era_type Γ Δ m n A).
 
 Lemma era_dyn_type Γ Δ m m' A :
-  Γ ; Δ ⊨ m ~ m' : A -> Γ ; Δ ⊨ m : A.
+  Γ ; Δ ⊢ m ~ m' : A -> Γ ; Δ ⊢ m : A.
 Proof with eauto using dyn_type. elim... Qed.
 
 Lemma dyn_era_type Γ Δ m A :
-  Γ ; Δ ⊨ m : A -> exists m', Γ ; Δ ⊨ m ~ m' : A.
+  Γ ; Δ ⊢ m : A -> exists m', Γ ; Δ ⊢ m ~ m' : A.
 Proof with eauto using era_type.
   elim=>{Γ Δ m A}.
   { move=>Γ Δ x A shs dhs. exists (Var x)... }
